move lemma to AST

backend/Inlining.v
@@ -465,3 +465,30 @@ Definition transf_program (p: program): Errors.res program :=
   let fenv := funenv_program p in
   AST.transform_partial_program (transf_fundef fenv) p.
 
+(** *For static renaming: transf_fundef and alpha are commute *)
+
+Definition transf_fundef_ctx ctx f := transf_fundef (funenv_program ctx) f.
+
+
+Lemma transf_function_alpha_commute: forall f f' ctx a,
+    transf_function (funenv_program ctx) f = OK f' ->
+    transf_function (funenv_program (alpha_rename a ctx)) (alpha_rename a f) = OK (alpha_rename a f').
+Proof.
+  unfold transf_function.
+    
+Admitted.
+
+Theorem transf_fundef_alpha_commute: forall fd fd' ctx a,
+    transf_fundef_ctx ctx fd = OK fd' ->
+    transf_fundef_ctx (alpha_rename a ctx) (alpha_rename a fd) = OK (alpha_rename a fd').
+Proof.
+  unfold transf_fundef_ctx. unfold transf_fundef.
+  intros. Transparent Alpha_fundef.
+  destruct fd;destruct fd'.
+  - simpl in *.
+    monadInv H.
+    admit. 
+  - simpl in H. monadInv H.
+  - simpl in H. monadInv H.
+  - simpl. auto.
+Admitted.
