common/Linking.v
@@ -577,109 +577,6 @@ Qed.
 
 (** *for static renaming *)
 
-(* some general lemma for PTree *)
-(* a general lemma for list *)
-Lemma in_list_first {A: Type} (Dec: forall (x y : A), {x=y} + {x<>y}):  forall (a:A) l,
-    In a l ->
-    exists l1 l2, l = l1 ++ a :: l2 /\ ~In a l1.
-Proof.
-  intros.
-  induction l.
-  simpl in H. contradiction.
-  simpl in H. destruct H.
-  exists (@nil A). exists l. simpl. rewrite H. auto.
-  destruct (Dec a a0).
-  exists (@nil A). exists l. simpl. rewrite e. auto.
-  apply IHl in H.
-  destruct H as [l1 [l2 [? ?]]].
-  exists (a0::l1). exists l2.
-  rewrite H. simpl. split. auto.
-  red. intros. destruct H1.
-  subst;congruence.
-  contradiction.
-Qed.
-
-Lemma in_list_last {A: Type} (Dec: forall (x y : A), {x=y} + {x<>y}) : forall (a:A) l,
-    In a l ->
-    exists l1 l2, l = l1 ++ a :: l2 /\ ~In a l2.
-Proof.
-  intros.
-  eapply in_rev in H.
-  eapply (in_list_first) in H;auto.
-  destruct H as [l1 [l2 [? ?]]].
-  exists (rev l2). exists (rev l1).
-  eapply rev_eq_app in H.
-  rewrite H. simpl.
-  rewrite<-app_assoc. simpl.
-  split;auto.
-  red. intros. apply in_rev in H1. contradiction.
-Qed.
-
-Lemma list_app_last {A: Type}: forall (l:list A) n , 
-    length l = S n ->
-    exists a l1 , l = l1 ++ (a::nil)  /\ length l1 = n. 
-Proof.
-  intros.
-  rewrite <- rev_length in H.
-  destruct (rev l) eqn: Rev.
-  simpl in H. congruence.
-  exists a ,(rev l0).
-  simpl in H. inversion H. 
-  split. assert (rev (rev l) = rev (a::l0)). f_equal. auto.
-  rewrite rev_involutive in H0.
-  rewrite H0. simpl. auto.
-  apply rev_length.
-Qed.
-
-Lemma PTree_fold_last_position_aux {V: Type} : forall n l b k (v:V),
-    length l = n ->
-    b ! k = None ->
-    (fold_left (fun (m : PTree.t V) (k_v : PTree.elt * V) =>
-                  PTree.set (fst k_v) (snd k_v) m) 
-               l b) ! k = Some v ->
-    exists l1 l2, l = l1 ++ (k,v) :: l2 /\ ~ In k (map fst l2). 
-Proof.
-  induction n.
-  - simpl. intros.
-    rewrite length_zero_iff_nil in H. subst.
-    simpl in *. rewrite H0 in H1. inversion H1.
-  - intros.
-    apply list_app_last in H.
-    destruct H as [a [l1 [? ?]]].
-    subst. erewrite  fold_left_app in H1.
-    simpl in H1.
-    destruct a. simpl in *.
-    (* discuss whether a equal to (k,v) *)
-    destruct (Pos.eq_dec e k).
-    + subst. erewrite PTree.gss in H1.
-      inversion H1. exists l1, nil.
-      simpl. auto.
-    + erewrite PTree.gso in H1;auto.
-      eapply IHn in H1.
-      destruct H1 as [l2 [l3 [? ?]]].
-      subst.
-      exists l2,(l3 ++ (e,v0)::nil).
-      rewrite <- app_assoc. split;auto.
-      red. intros. apply H1.
-      rewrite map_app in H.
-      eapply in_app in H.
-      destruct H. auto. simpl in H. destruct H;auto.
-      congruence. contradiction.
-      auto.
-      auto.
-Qed.
-
-Lemma PTree_of_list_last_position {V: Type} : forall l k (v:V),
-    (PTree_Properties.of_list l) ! k = Some v ->
-    exists l1 l2, l = l1 ++ (k,v) :: l2 /\ ~ In k (map fst l2).
-Proof.
-  unfold PTree_Properties.of_list.
-  intros.
-  eapply PTree_fold_last_position_aux.
-  auto.
-  apply PTree.gempty.
-  auto.
-Qed.
 
 Theorem alpha_partial_program_match:
   forall {A B V: Type} {LA: Linker A} {LV: Linker V}
@@ -780,113 +677,6 @@ Proof.
   apply linkorder_refl. intros. auto.
 Qed.
 
-(* add to AST.v *)
-Lemma exists_inverse_permutation : forall (a:permutation),
-    exists b, inverse_permutation a b.
-Admitted.
-
-Lemma inverse_permutation_sym : forall a b,
-    inverse_permutation a b -> inverse_permutation b a.
-  Admitted.
-
-(* a general lemma for PTree, hard to prove! *)
-Lemma Bijective_Injective {A B: Type}: forall (f: A->B), FinFun.Bijective f -> FinFun.Injective f.
-Proof.
-  unfold FinFun.Bijective. unfold FinFun.Injective.
-  intros.
-  destruct H as [g [? ?]].
-  eapply f_equal in H0.
-  erewrite H in H0.  erewrite H in H0.
-  auto.
-Qed.
-
-Lemma PTree_of_list_map {V: Type} : forall (f: positive -> positive) (g: V -> V) (l:list (positive * V)) k (v: V),
-    (FinFun.Bijective f) ->
-    (PTree_Properties.of_list l) ! k = Some v ->
-    (PTree_Properties.of_list
-       (map (fun (ele:(positive*V)) =>  (f (fst ele), g (snd ele))) l)) ! (f k) = Some (g v).
-Proof.
-  intros.
-  induction l.
-  - unfold PTree_Properties.of_list in *.
-    simpl in *.
-    erewrite PTree.gempty in H0.
-    inversion H0.
-  - intros.
-    (* key idea : discuss whether a in l or not, because of_list take the last occurence *)
-    destruct (in_dec Pos.eq_dec k (map fst l)).
-    + apply PTree_of_list_last_position in H0.
-      destruct H0 as [l1 [l2 [? ?]]].
-      destruct l1.
-      * rewrite H0. simpl in *.
-        rewrite <- (app_nil_l ((f k, g v)
-      :: map (fun ele : positive * V => (f (fst ele), g (snd ele)))
-           l2)).
-        eapply PTree_Properties.of_list_unique.
-        erewrite map_map. simpl.
-        (* f is Bijective *)
-        unfold FinFun.Bijective in H. destruct H as [f1 [? ?]].
-        red. intros. eapply (in_map f1) in H3.
-        erewrite H in H3. erewrite map_map in H3.
-        apply H1. erewrite <- map_id. (* use map_id to solve lta conversion *)
-        erewrite map_map. clear H0 IHl H1.
-        induction l2.
-        simpl in H3. auto.
-        simpl in *. destruct H3.
-        left. erewrite H in H0. auto.
-        right. apply IHl2. auto.
-      * simpl in H0. injection H0. intros;subst.
-        clear H0. rewrite app_comm_cons.
-        rewrite map_app. simpl.
-        rewrite app_comm_cons.
-        eapply PTree_Properties.of_list_unique.
-        erewrite map_map. simpl.
-        unfold FinFun.Bijective in H. destruct H as [f1 [? ?]].
-        red. intros. eapply (in_map f1) in H2.
-        erewrite H in H2. erewrite map_map in H2.
-        apply H1. erewrite <- map_id. (* use map_id to solve lta conversion *)
-        erewrite map_map. clear IHl H1 i.
-        induction l2.
-        simpl in H2. auto.
-        simpl in *. destruct H2.
-        left. erewrite H in H1. auto.
-        right. apply IHl2. auto.
-    + eapply PTree_Properties.in_of_list in H0. simpl in H0.
-      destruct H0.
-      * subst.
-        assert (~ In (f k) (map f (map fst l))).
-        { erewrite map_map.
-          red.
-          erewrite in_map_iff.
-          intros. destruct H0 as [x [? ?]].
-          apply Bijective_Injective in H. unfold FinFun.Injective in H.
-          eapply H in H0.
-          apply (in_map fst) in H1. rewrite H0 in H1. auto.
-        }.
-        simpl. rewrite <- (app_nil_l ((f k, g v)
-      :: map (fun ele : positive * V => (f (fst ele), g (snd ele))) l)).
-        eapply PTree_Properties.of_list_unique.
-        erewrite map_map. erewrite map_map in H0.
-        simpl. auto.       
-      * apply (in_map fst) in H0.
-        simpl in H0. contradiction.
-Qed.
-
-        
-(* a more general lemma, need to be moved to AST.v *)
-Lemma rename_program_remain_gd {F V: Type} {AF: Alpha F} {AV: Alpha V}: forall (p:AST.program F V) id gd a,
-    (prog_defmap p) ! id = Some gd ->
-    (prog_defmap (alpha_rename a p)) ! (alpha_rename a id) = Some (alpha_rename a gd).
-Proof.
-  unfold prog_defmap.
-  Transparent Alpha_prog.
-  destruct p. simpl in *.
-  intros. eapply PTree_of_list_map.
-  destruct a. simpl. auto.
-  auto.
-Qed.
-
-
 
 Lemma linkorder_alpha {A V:Type} {LA: Linker A} {LV: Linker V} {ALA: Alpha A}  {ALV: Alpha V}:
   forall (p1 p2:program A V) a,
@@ -901,14 +691,14 @@ Proof.
   split.
   - apply incl_map. auto.
   - intros.
-    generalize (exists_inverse_permutation a).
+    assert (exists b, inverse_permutation a b) by eapply exists_inverse_permutation.
     intros. destruct H3 as [b ?].
-    eapply (rename_program_remain_gd _ _ _ b) in H2.
+    eapply (rename_program_remain_gd _ _ b) in H2.
     assert ((alpha_rename b (alpha_rename_prog a p1)) = p1).
     { erewrite alpha_rename_sym. auto. simpl. auto. auto. }
     rewrite H4 in *. apply H1 in H2. clear H1 H0.
     destruct H2 as [gd2 [? [? ?]]].
-    eapply (rename_program_remain_gd _ _ _ a) in H0. 
+    eapply (rename_program_remain_gd _ _  a) in H0. 
     erewrite alpha_rename_sym in H0. 2: reflexivity. 2: auto.
     simpl in H0. exists (alpha_rename a gd2).
     split.
